proof/Poly/Exp.v
@@ -1,8 +1,17 @@
 
-Require Import Ty.
-Require Import Env.
-Require Import Base.
-Require Import SubstTypeType.
+(* Kinds ************************************************************)
+Inductive ki : Type :=
+ | KStar   : ki.
+
+
+(** Types ***********************************************************)
+Inductive ty  : Type :=
+ | TCon    : nat -> ty
+ | TVar    : nat -> ty
+ | TForall : ty  -> ty
+ | TFun    : ty  -> ty -> ty.
+Hint Constructors ty.
+
 
 (** Expressions *****************************************************)
 Inductive exp : Type :=
@@ -12,33 +21,4 @@ Inductive exp : Type :=
  | XLam  : ty  -> exp -> exp
  | XApp  : exp -> exp -> exp.
 Hint Constructors exp.
-
-
-(* Well Formedness **************************************************)
-
-(* Exp is closed under the given environments *)
-Fixpoint wfX (kenv: env ki) (tenv: env ty) (xx: exp) : Prop := 
- match xx with 
- | XVar i     => exists t, get tenv i = Some t
- | XLAM x     => wfX (kenv :> KStar) tenv x
- | XAPP x t   => wfX kenv tenv x  /\ wfT kenv t
- | XLam t x   => wfT kenv t       /\ wfX kenv (tenv :> t) x
- | XApp x1 x2 => wfX kenv tenv x1 /\ wfX kenv tenv x2
- end.
-Hint Unfold wfX.
-
-
-(* Closed expressions are well formed under empty environments *)
-Definition closedX (xx: exp) : Prop
- := wfX Empty Empty xx.
-Hint Unfold closedX.
-
-
-(* Values are closed expressions that cannot be reduced further *)
-Inductive value : exp -> Prop :=
- | Value_lam 
-   : forall t x
-   , closedX (XLam t x) -> value (XLam t x).
-Hint Constructors value.
-
 
