proof/Poly/WellFormed.v
@@ -1,0 +1,61 @@
+
+Require Import Exp.
+Require Import TyEnv.
+
+
+(* Types ************************************************************)
+(* Well formed types are closed under the given kind environment *)
+Fixpoint wfT (e: tyenv) (tt: ty) : Prop := 
+ match tt with
+ | TCon _     => True
+ | TVar i     => exists k, getK e i = Some k
+ | TForall t  => wfT (e :> EKind KStar) t
+ | TFun t1 t2 => wfT e t1 /\ wfT e t2
+ end.
+Hint Unfold wfT.
+
+
+(* Type is closed under an empty kind environment. *)
+Definition closedT (tt: ty) : Prop
+ := wfT Empty tt.
+Hint Unfold closedT.
+
+
+(* Environments ****************************************************)
+(* All types in a well formed environment are well formed under
+   the subsequent environment 
+ *)
+Fixpoint wfEnv (e: tyenv) : Prop :=
+ match e with 
+ | Empty         => True
+ | e' :> EKind _ => wfEnv e'
+ | e' :> EType t => wfT e' t /\ wfEnv e'
+ end.
+
+
+(* Expressions ******************************************************)
+(* A well formed expression is closed under the given environment *)
+Fixpoint wfX (e: tyenv) (xx: exp) : Prop := 
+ match xx with 
+ | XVar i     => exists t, getT e i = Some t
+ | XLAM x     => wfX (e :> EKind KStar) x
+ | XAPP x t   => wfX e x  /\ wfT e t
+ | XLam t x   => wfT e t  /\ wfX (e :> EType t) x
+ | XApp x1 x2 => wfX e x1 /\ wfX e x2
+ end.
+Hint Unfold wfX.
+
+
+(* Closed expressions are well formed under empty environments *)
+Definition closedX (xx: exp) : Prop
+ := wfX Empty xx.
+Hint Unfold closedX.
+
+
+(* Values are closed expressions that cannot be reduced further *)
+Inductive value : exp -> Prop :=
+ | Value_lam 
+   : forall t x
+   , closedX (XLam t x) -> value (XLam t x).
+Hint Constructors value.
+
